---
title: "Lesson 1.1"
subtitle: "The Cumulative Distribution Function Technique"
format: pdf
editor: visual
font: 12px
---

## Introduction

The objective of statistics is to make inferences about a population based on information contained in a sample taken from that population. The quantities used to estimate population parameters or to make decisions about a population are functions of the $n$ random observations that appear in a sample.

To illustrate, consider the problem of estimating a population mean, $\mu$. Intuitively, we draw a random sample of $n$ observations, $y_1, y_2, \ldots , y_n$, from the population and use the sample mean $$
\bar{Y} = \frac{\sum_{i=1}^n Y_i}{n}
$$

to estimate $\mu$.

If the probability distributuion of the $Y_i's$ is known what would be the distribution of the sample mean $\bar{Y}$. If $Y_i's$ are random variables then $\bar{Y}$ is likewise a random variable.

In this module, we shall study methods in finding the distribution of functions of random variables. These methods include:

1.  Cumulative Distribution Function (CDF) Technique

2.  Transformation Technique

3.  Moment Generation Function (MGF) Technique

## The Cumulative Distribution Function (CDF) Technique

Suppose $Y$ is a continuous random variable with cumulative distribution function $F_Y(y) = P(Y \leq y)$. The CDF technique is useful if $F_Y(y)$ has a closed form. The steps in the CDF method are:

1.  Find a closed form of the CDF of $Y$.

2.  Find the support of $U=g(Y)$.

3.  Write $F_U(u) = P(U \leq U)$ in terms of $F)Y(y)$.

4.  Differentiate $F_U(u)$ to obtain the PDF of $U$.

### Example 1.1.1

Suppose $Y \sim U(0,1)$. Find the distribution of $U = g(Y) = -lnY$.

**SOLUTION**

Verify that the CDF of Y is given by

$$
F_Y(y) = \begin{cases}
0, \, y \leq 0 \\
y,\, 0< y < 1 \\
1, \, y \geq 1
\end{cases}
$$

Since the support for $Y \sim U(0,1)$ is $R_Y = \{y: 0 < y <1 \}$, thus, it follows that the support for $U = -ln Y$ is $R_U = \{u: u >0 \}$.

Now, we are going to find the CDF of $U$.

$$
\begin{aligned}
F_U(u) &= P(U \leq u) \\
&= P(-lnY \leq u) \\
&= P(lnY > -u) \\
&= P(Y > e^{-u}) \\
&= 1- P(Y \leq e^{-u}) \\
&= 1- F_Y(e^{-u})
\end{aligned}
$$

Since $F_Y(y) = y$ for $0 < y < 1$, hence, for $u >0$ we have

$$
\begin{aligned}
F_U(u) &= 1- F_Y(e^{-u}) \\
&= 1 - e^{-u}
\end{aligned}
$$

To get the PDF of $U$, we have

$$
\begin{aligned}
f_U(u) &= \frac{d}{du} F_U(u) \\
&= \frac{d}{du} \left[1- e^{-u} \right] \\
&= e^{-u}
\end{aligned}
$$

Therefore,

$$
f_U(u) = \begin{cases}
e^{-u}, \; u > 0 \\
0,\, \text{elsewhere}
\end{cases}
$$

which shows that $U \sim Exp(1)$ which is an exponential distribution with mean $\beta = 1$.

### Example 1.1.2

A process for refining sugar yields up to 1 ton of pure sugar per day, but the actual amount produced, $Y$, is a random variable because of machine breakdowns and other slowdowns. Suppose that $Y$ has density function given by

$$
f_Y(y) = \begin{cases}
2y,\, 0 \leq y \leq 1 \\
0,\, \text{elsewhere}
\end{cases}
$$

The company is paid at the rate of \$300 per ton for the refined sugar, but it also has a fixed overhead cost of \$100 per day. Thus the daily profit, in hundreds of dollars, is $U = 3Y âˆ’ 1$. Find the probability density function for $U$.

**SOLUTION**

Verify that the CDF of $Y$ is given by

$$
F_Y(y) = \begin{cases}
0,\, y < 0 \\
y^2,\, 0 \leq y < 1 \\
1, \, y \geq 1
\end{cases}
$$

Note that the support of $U = 3Y - 1$ is $R_U = \{u: -1 \leq u \leq 2 \}$.

The CDF of $U$ is obtained as follows:

$$
\begin{aligned}
F_U(u) &= P(U \leq u) \\
&= P(3Y - 1 \leq u) \\
& = P(Y \leq \frac{u + 1}{3}) \\
&= F_Y\left(\frac{u + 1}{3}\right)
\end{aligned}
$$

That is, for $-1 \leq u \leq 2$,

$$
\begin{aligned}
F_U(u) &= F_Y\left(\frac{u + 1}{3}\right) \\
&= \left(\frac{u + 1}{3}\right)^2
\end{aligned}
$$

And the density function for $U$ is

$$
\begin{aligned}
f_U(u) &= \frac{d}{du} F_U(u) \\
&= \frac{d}{du} \left[ \left(\frac{u + 1}{3}\right)^2\right] \\
&= \frac{2}{9} (u + 1)
\end{aligned}
$$

Therefore, $$
f_U(u) = \begin{cases}
\frac{2}{9} (u + 1), \; -1 \leq u \leq 2 \\
0,\, \text{elsewhere}
\end{cases}
$$

### Example 1.1.3

Let $Y$ be a random variable with PDF

$$
f_Y(y) = \begin{cases}
\frac{3}{2} y^2,\, -1 \leq y \leq 1 \\
0,\, \text{elsewhere}
\end{cases}
$$

**SOLUTION** \[Left as a classroom exercise!\]
